\documentclass[12pt,fleqn]{article}\usepackage{../../common}
\begin{document}

$$ \kappa(1-\omega-rd)= v (\alpha + \beta + \delta)$$

$$ \overline{\pi}_1 = 1-\omega-rd  $$

$$ d = \frac{1-\overline{\pi}_1-\omega}{r} $$

$$ 
\dot{d} = d \bigg[
r - \frac{\kappa(1-\omega-rd)}{v} + \delta
\bigg] + \kappa(1-\omega-rd) - (1-\omega)
\mlabel{4}
$$


$$ 
0 =  \frac{1-\overline{\pi}_1-\omega}{r} \bigg[
r - \frac{v (\alpha + \beta + \delta)}{v} + \delta
\bigg] + v (\alpha + \beta + \delta)- 1+\omega
$$

$$ 
-\omega =  \bigg(\frac{1}{r}-\frac{\overline{\pi}_1}{r}-\frac{\omega}{r}\bigg) \bigg(
r - \alpha + \beta + \delta + \delta
\bigg) + v (\alpha + \beta + \delta)- 1
$$

$$ 
-\omega =
\bigg(\frac{1}{r}-\frac{\overline{\pi}_1}{r}-\frac{\omega}{r}\bigg)c_1 +
c_2 - 1
$$

$$ 
-\omega = \frac{c_1}{r}-\frac{c_1\overline{\pi}_1}{r}-\frac{c_1 \omega}{r}  +c_2 - 1
$$

$$ 
-\omega(\frac{c_1 }{r} -1) = \frac{c_1}{r}-\frac{c_1 \overline{\pi}_1}{r} +c_2 - 1
$$

$$ 
-\omega(\frac{c_1-r }{r}) = \frac{c_1 - c_1 \overline{\pi}_1 + rc_2 - r}{r}
$$

$$ 
-\omega = \frac{c_1 - c_1\overline{\pi}_1 + rc_2 - r}{c_1 - r}
$$







$$ \omega = 1-\pi_1-r \frac{v(\alpha+\beta+\delta) - \pi_1}{\alpha+\beta}$$




















\end{document}






