\documentclass[12pt,fleqn]{article}\usepackage{../../common}
\begin{document}
Fonksiyonel Optimizasyonu

\begin{minted}[fontsize=\footnotesize]{python}
import sympy

t = sympy.symbols('t')
x = sympy.Function('x')
diffeq = sympy.Eq(x(t).diff(t, t) - 2*x(t),0)
print (sympy.latex (sympy.dsolve(diffeq, x(t))))
\end{minted}

\begin{verbatim}
x{\left(t \right)} = C_{1} e^{- \sqrt{2} t} + C_{2} e^{\sqrt{2} t}
\end{verbatim}

$$
x{\left(t \right)} = C_{1} e^{- \sqrt{2} t} + C_{2} e^{\sqrt{2} t}
$$

\begin{minted}[fontsize=\footnotesize]{python}
diffeq = sympy.Eq(x(t).diff(t, t) - 2*x(t),0)
solved = sympy.dsolve(diffeq, x(t), ics={x(0):1,x(1):0 } ) 
solved = sympy.simplify(solved)
print (sympy.latex (solved))
\end{minted}

\begin{verbatim}
x{\left(t \right)} = \frac{\left(e^{2 \sqrt{2} t} - e^{2 \sqrt{2}}\right) e^{- \sqrt{2} t}}{1 - e^{2 \sqrt{2}}}
\end{verbatim}

$$
x{\left(t \right)} = \frac{\left(e^{2 \sqrt{2} t} - e^{2 \sqrt{2}}\right) e^{- \sqrt{2} t}}{1 - e^{2 \sqrt{2}}}
$$



%x=dsolve('D2x-2*x=O','x(O)=1,x(1)=O')












\end{document}
